theories/iris/logrel/instr/typing/store_weak.v
@@ -13,6 +13,28 @@ Section store_weak.
   Variable sr : store_runtime.
   Variable mr : module_runtime.
 
+  (* TEMPORARY. This is a copy. *)
+  Lemma rep_ref_kind_ptr_TEMP F κ μ τ ρ ξ :
+    has_kind F (RefT κ μ τ) (VALTYPE ρ ξ) ->
+    ρ = AtomR PtrR /\ exists ξ', κ = VALTYPE (AtomR PtrR) ξ'.
+  Proof.
+    intros Hkind.
+    remember (RefT κ μ τ) as ref.
+    remember (VALTYPE ρ ξ) as val.
+    revert Heqval Heqref.
+    revert ρ ξ.
+    induction Hkind using has_kind_ind'; intros; try congruence.
+    - subst κ0.
+      split; try congruence.
+      inversion Heqref; eauto.
+    - subst κ0.
+      split; try congruence.
+      inversion Heqref; eauto.
+    - subst κ'.
+      inversion H; subst; eapply IHHkind; eauto.
+  Qed.
+
+
   Lemma compat_store_weak M F L wt wt' wtf wl wl' wlf es' κ κser μ τ τval π pr :
     let fe := fe_of_context F in
     let WT := wt ++ wt' ++ wtf in
@@ -29,17 +51,15 @@ Section store_weak.
   Proof.
     intros fe WT WL lmask ψ Hresolves Hdrop Hser Hmonosize Htype Hcompile.
     unfold WT, WL; clear WT WL.
-    (* If the WT := or WL := become necessary, undo the unfold/clear*)
     cbn in Hcompile.
 
-    (* Mechanically get through some of the first few things in compile_swap *)
     inv_cg_bind Hcompile ρ ?wt ?wt ?wl ?wl es_off ?es_rest Hρ Hcompile.
     inv_cg_bind Hcompile ιs ?wt ?wt ?wl ?wl es_ρ ?es_rest Hιs Hcompile.
     inv_cg_bind Hcompile off ?wt ?wt ?wl ?wl  es_fail ?es_rest Hoff Hcompile.
     inv_cg_try_option Hρ; rename Heq_some into Hρ.
     inv_cg_try_option Hιs; rename Heq_some into Hιs.
     inv_cg_try_option Hoff; rename Heq_some into Hoff.
-    inv_cg_bind Hcompile vs ?wt ?wt ?wl ?wl  es_save ?es_rest Hsave Hcompile.
+    inv_cg_bind Hcompile lcidxs ?wt ?wt ?wl ?wl  es_save ?es_rest Hsave Hcompile.
     inv_cg_bind Hcompile a ?wt ?wt ?wl ?wl  es_a ?es_rest Ha Hcompile.
     cbn in Ha; inversion Ha; subst; clear Ha.
     inv_cg_bind Hcompile res_emit ?wt ?wt ?wl ?wl  es_emit ?es_rest Hemit Hcompile.
@@ -48,9 +68,151 @@ Section store_weak.
 
     (* Some clean up *)
     subst.
-    (* clear_nils. *)
+    clear_nils.
+    destruct u. destruct p; destruct u; destruct u0.
 
-    (* The next step is a case_ptr, for which a lemma is currently being proven about *)
+    (* Let's dig into some of the atoms/values that are floating around *)
+    unfold have_instr_type_sem.
+    iIntros (??????????) "@@@@@@@@@".
+    iPoseProof (values_interp_cons_l with "[$Hos]") as "(%os1 & %os2 & -> & Hos1 & Hos2)".
+    iEval (rewrite values_interp_one_eq; cbn) in "Hos2".
+    iPoseProof (atoms_interp_app_l with "[$Hvs]") as "(%vs1 & %vs2 & -> & Hvs1 & Hvs2)".
+    iPoseProof (value_interp_ref_sz with "[$Hos1]") as "%Hos1len".
+    destruct os1; [inversion Hos1len | destruct os1; [| inversion Hos1len]].
+    rename a into o1.
+    iEval (rewrite atoms_interp_one_inv) in "Hvs1".
+    iDestruct "Hvs1" as "(%v1 & -> & Hv1)".
+    set (ptr_local := sum_list_with length (typing.fc_locals F) + length (wl ++ wl6) ) in *.
+    iEval (rewrite value_interp_eq) in "Hos1".
+    iDestruct "Hos1" as (κ' Hκ') "[Harepos1 Hrefos1]".
+    destruct κ'; [|by iDestruct "Harepos1" as "[[] ?]"].
+    iDestruct "Harepos1" as "%Harepos1".
+    cbn in Hκ'.
+
+
+    assert (Hκ: eval_rep se (AtomR PtrR) = Some l).
+    {
+      inversion Htype as [? ? ? Hmono Hctx]; subst.
+      destruct Hmono as [Hmono _].
+      rewrite Forall_cons in Hmono.
+      destruct Hmono as [Hmono Hmonoτval].
+      rewrite Forall_singleton in Hmonoτval.
+      inversion Hmono as [? ? ? Hrep Hismono]; subst.
+      inversion Hrep; subst.
+      apply rep_ref_kind_ptr_TEMP in H1; subst.
+      destruct H1 as [-> [χ' ->]].
+      unfold eval_kind in Hκ'.
+      apply bind_Some in Hκ'; destruct Hκ' as [l' [Heval Hret]].
+      inversion Hret; subst; auto.
+    }
+    cbn in Hκ; inversion Hκ; subst l.
+    unfold has_areps in Harepos1.
+    destruct Harepos1 as [[os1' [Hos1 Harepsos1]] Hrefflag].
+    inversion Hos1; subst os1'; clear Hos1. clear Hκ.
+    apply Forall2_cons_1 in Harepsos1 as [Harepo1 _].
+    destruct o1; inversion Harepo1.
+    apply has_values_app_inv in H0 as (evs1 & evs2 & Hevs & Hevs1 & Hevs2).
+    pose proof (has_values_length _ _ Hevs1) as Hlenevs1.
+    destruct evs1 as [|ev1 [|evvv' evvvs]]; try (cbn in *; congruence).
+    iPoseProof (frame_interp_wl_interp with "Hframe") as "%Hwl"; first done.
+    subst.
+    (* clearing some useless things *)
+    clear Hlenevs1 Hos1len.
+    rewrite (app_assoc ([ev1] ++ evs2)).
+    iApply (cwp_seq with "[Hfr Hrun]").
+    {
+      rewrite <- (app_assoc [ev1]).
+     (* instantiate (1 := λ f vs, (
+        ⌜vs = [v1]⌝ ∗
+        ⌜∀ i, i ∉ lcidxs -> f_locs f !! localimm i = f_locs fr !! localimm i⌝ ∗
+        ⌜Forall2 (fun i v => f_locs f !! localimm i = Some v) lcidxs vs2⌝
+        )%I).*)
+      instantiate (1 := λ fr' vs, (
+        ∃ val_idxs,
+        ⌜vs = [v1]⌝ ∗
+        ⌜frame_rel (λ i, i ∉ val_idxs) fr fr'⌝ ∗
+        ⌜Forall2 (fun i v => f_locs fr' !! localimm i = Some v) lcidxs vs2⌝ ∗
+        ⌜val_idxs = seq (fe_wlocal_offset fe + length wl) (length wl6)⌝ ∗
+        ⌜lcidxs = map prelude.W.Mk_localidx val_idxs⌝
+        )%I).
+
+      iApply cwp_val_app; first done.
+      set (temp := map prelude.W.Mk_localidx
+                        (seq (fe_wlocal_offset fe + length wl)
+                           (length (map translate_prim (map arep_to_prim ιs))))) in *.
+
+      eapply cwp_save_stack_w in Hsave.
+      4: {
+        apply Hevs2.
+      }
+      2: apply Hwl.
+      + destruct Hsave as (-> & -> & -> & Hsave).
+        (*iApply (Hsave with "[$] [$]").
+        iIntros (f' [Hfsame Hfchanged]).
+        unfold fvs_combine; done.*) admit.
+      + admit.
+      + admit.
+    }
+
+    iIntros (fr_saved w)
+      "(%val_idxs & -> & %Hfrel_fr_saved & %Hsaved & %Hval_idxs_seq & %Hval_localidxs) Hfr Hrun".
+
+    assert (ptr_local < length (f_locs fr_saved)) as Hlen.
+    {
+      admit.
+    }
+
+
+    simpl to_consts. iEval (rewrite app_assoc).
+
+    iApply (cwp_seq with "[Hfr Hrun]").
+    {
+      simpl app.
+      iApply (cwp_local_tee with "[ ] [$] [$]"); first auto.
+      admit.
+    }
+
+    (*
+    iIntros (f0 vs0) "[-> ->] Hfr Hrun".
+    eapply cwp_case_ptr in Hcompile.
+    2: do 2 instantiate (1 := []).
+    2,3: done.
+    destruct Hcompile as (?wt & ?wt & ?wt & ?wl & ?wl & ?wl & ?es & ?es & ?es & Hcompile).
+    destruct Hcompile as (Hunr & Hload1 & Hload2 & Hwt0 & Hwl0 & Hspec).
+
+
+
+
+    iApply cwp_val_app.
+    { instantiate (1 := [v1]).
+      apply Is_true_true.
+      apply/andP; split => //. by apply/eqP. }
+
+    iApply (cwp_seq with "[Hfr Hrun Hv1 Hrefos1]").
+    {
+      iApply (Hspec with "[$] [$] [] [$Hv1]").
+      {
+        iPureIntro; cbn. rewrite list_lookup_insert. by rewrite decide_True.
+      }
+      iIntros "!> Hfr Hrun Hv1".
+      clear_nils.
+      iEval (cbn) in "Hrefos1".
+      destruct μ as [|[|]]; first done.
+      - (* mm *)
+        unfold ref_mm_interp.
+        admit.
+      - (* gc *)
+        unfold ref_gc_interp.
+        admit.
+
+    }
+
+    iIntros (ff vss) "hi Hfr Hrun".
+    subst.
+     *)
+
+
+
   Admitted.
 
 End store_weak.
